ReductionSeq: standardize on yet another form of ReductionSeq

Thesis/ReductionSeq.lean
@@ -12,95 +12,47 @@ variable {α I}
 variable (A: ARS α I)
 
 /--
-`ReductionSeq A is x y` represents a reduction sequence in `A`,
-taking indexed reduction steps as given in `is` from `x` to `y`.
+`ReductionSeq A x y ss` represents a reduction sequence in `A`,
+taking indexed reduction steps as given in `ss` from `x` to `y`.
 
 An empty reduction sequence is represented by `ReductionSeq.refl`, allowing a
 reduction from `x` to `x` in 0 steps. Using `ReductionSeq.head`, a single step
 `a ⇒[i] b` can be prepended to an existing reduction sequence.
 -/
-inductive ReductionSeq: List I → α → α → Prop
-  | refl (x) : ReductionSeq [] x x
-  | head {i x y z} : A.rel i x y → ReductionSeq is y z → ReductionSeq (i :: is) x z
+inductive ReductionSeq: α → α → List (I × α) → Prop
+  | refl {x} : ReductionSeq x x []
+  | head {i x y} : A.rel i x y → ReductionSeq y z ss → ReductionSeq x z ((i, y)::ss)
 
-theorem ReductionSeq.tail (hr : ReductionSeq A l a b) (hstep : A.rel i b c) : ReductionSeq A (l ++ [i]) a c := by
+def ReductionSeq.elems (hseq: ReductionSeq A x y ss) := x :: (ss.map (·.2))
+
+theorem ReductionSeq.tail (hr: ReductionSeq A x y ss) (hstep: A.rel i y z) : ReductionSeq A x z (ss ++ [(i, z)]) := by
   induction hr with
-  | refl => apply head hstep; exact refl c
-  | head step _ ih => exact head step (ih hstep)
+  | refl => simp; apply head hstep; apply refl
+  | head step r ih =>
+    simp_all
+    apply head step
+    exact ih
 
-theorem ReductionSeq.concat : ReductionSeq A l x y → ReductionSeq A l' y z → ReductionSeq A (l ++ l') x z := by
-  intro r₁ r₂
-  induction r₁ with
-  | refl a => rwa [List.nil_append]
-  | head step _ ih => exact ReductionSeq.head step (ih r₂)
+theorem ReductionSeq.concat (h₁ : ReductionSeq A x y ss) (h₂: ReductionSeq A y z ss') : ReductionSeq A x z (ss ++ ss') := by
+  induction h₁ with
+  | refl => exact h₂
+  | head hstep hseq ih =>
+    apply head hstep (ih h₂)
 
 /-- A reduction sequence exists iff there is a reflexive-transitive reduction. -/
-lemma ReductionSeq.exists_iff_union_rel_star {x y : α} : A.union_rel∗ x y ↔ ∃is, ReductionSeq A is x y := by
+lemma ReductionSeq.exists_iff_union_rel_star {x y : α}: A.union_rel∗ x y ↔ ∃ss, ReductionSeq A x y ss := by
   constructor <;> intro r
   · induction r using ReflTransGen.head_induction_on with
-    | refl => use []; exact ReductionSeq.refl y
-    | head step _ ih =>
-        obtain ⟨is, h⟩ := ih
-        obtain ⟨i, h'⟩ := step
-        use (i :: is)
-        apply ReductionSeq.head h' h
-  · rcases r with ⟨is, r⟩
+    | refl => use [], ReductionSeq.refl
+    | head step seq ih =>
+        obtain ⟨ss', hss'⟩ := ih
+        obtain ⟨i, hi⟩ := step
+        exact ⟨_, head hi hss'⟩
+  · rcases r with ⟨ss, r⟩
     induction r with
-    | refl a => apply ReflTransGen.refl
-    | head step _ ih =>
-        apply ReflTransGen.head
-        · exact Exists.intro _ step
-        · exact ih
-
-
-/-- A more complicated version of ReductionSeq that includes all of the elements. -/
-inductive ReductionSeq': List I → List α → α → α → Prop
-  | rel {i x y} : A.rel i x y → ReductionSeq' [i] [x, y] x y
-  | head {i x y z} : A.rel i x y → ReductionSeq' is as y z → ReductionSeq' (i::is) (x::as) x z
-
-theorem ReductionSeq'.tail (hr: ReductionSeq' A is as x y) (hstep: A.rel i y z) : ReductionSeq' A (is ++ [i]) (as ++ [z]) x z := by
-  induction hr with
-  | rel hr => apply head hr; exact rel hstep
-  | head step _ ih => apply head step; apply ih; simp_all only [List.cons_append, List.getLast?_cons_cons]
-
-theorem ReductionSeq'.concat (h₁ : ReductionSeq' A is as x y) (h₂: ReductionSeq' A is' (y::as') y z) : ReductionSeq' A (is ++ is') (as ++ as') x z := by
-  induction h₁ with
-  | rel hr => apply head hr; exact h₂
-  | head step _ ih => apply head step (ih h₂)
-
-lemma ReductionSeq'.as_last : ReductionSeq' A is as x y → ∃as', as = (as' ++ [y]) := by
-  intro hr
-  induction hr with
-  | rel h => rename_i i x y; use [x]; rfl
-  | head h h' ih => rename_i is as i x y z; obtain ⟨as', has'⟩ := ih; use (x::as'); simp_all only [List.cons_append]
-
-lemma ReductionSeq'.as_head : ReductionSeq' A is as x y → ∃as', as = (x::as') := by
-  intro hr; cases hr; use [y]; simp
-
-/-- A reduction sequence exists iff there is a nonempty reflexive-transitive reduction. -/
-lemma ReductionSeq'.exists_iff_union_rel_star {x y : α} (hne: x ≠ y): A.union_rel∗ x y ↔ ∃is as, ReductionSeq' A is as x y := by
-  constructor <;> intro r
-  · induction r using ReflTransGen.head_induction_on with
-    | refl => contradiction
-    | head step _ ih =>
-        rename_i a c h
-        obtain ⟨i, h'⟩ := step
-        by_cases hc: (c = y)
-        · rw [<-hc]
-          use [i], [a, c]; exact rel h'
-        · simp [hc] at ih
-          obtain ⟨is, ⟨as, h⟩⟩ := ih
-          use (i :: is), (a :: as)
-          apply head h' h
-  · rcases r with ⟨is, as, r⟩
-    clear hne
-    induction r with
-    | rel a => rename_i i x y; apply ReflTransGen.single; use i
-    | head step h ih =>
-        rename_i is as i x y z
-        apply ReflTransGen.head
-        · exact Exists.intro _ step
-        · exact ih
+    | refl => rfl
+    | head step seq ih =>
+      exact ReflTransGen.head ⟨_, step⟩ ih
 
 
 end reduction_seq
